intro, elim, fold_recursive

src/lowparse/LowParse.SteelST.Recursive.fst
@@ -664,3 +664,492 @@ let jump_recursive
   let _ = gen_elim () in
   noop ();
   return res
+
+let get_children
+  (#p: parse_recursive_param)
+  (s: serialize_recursive_param p)
+  (x: p.t)
+: Tot (list p.t)
+= dsnd (s.synth_recip x)
+
+module LPC = LowParse.SteelST.Combinators
+module NL = LowParse.SteelST.VCList
+
+let intro_recursive_as_nlist
+  (#opened: _)
+  (p: parse_recursive_param)
+  (#vl: v p.parse_header_kind p.header)
+  (n: nat)
+  (al: byte_array)
+  (#vr: v (parse_nlist_kind n (parse_recursive_kind p.parse_header_kind)) (nlist n p.t))
+  (ar: byte_array)
+: STGhost (v (parse_recursive_kind p.parse_header_kind) p.t) opened
+    (aparse p.parse_header al vl `star`
+      aparse (parse_nlist n (parse_recursive p)) ar vr
+    )
+    (fun va -> aparse (parse_recursive p) al va)
+    (AP.adjacent (array_of vl) (array_of vr) /\
+      n == p.count vl.contents
+    )
+    (fun va ->
+      AP.merge_into (array_of vl) (array_of vr) (array_of va) /\
+      n == p.count vl.contents /\
+      va.contents == p.synth_ (| vl.contents, vr.contents |)
+    )
+= let _ = LPC.intro_dtuple2 p.parse_header (parse_recursive_payload p (parse_recursive p)) al ar in
+  let _ = LPC.intro_synth _ p.synth_ al () in
+  Classical.forall_intro (parse_recursive_eq p);
+  rewrite_aparse al (parse_recursive p)
+
+let intro_recursive_as_list
+  (#opened: _)
+  (p: parse_recursive_param)
+  (#vl: v p.parse_header_kind p.header)
+  (al: byte_array)
+  (#vr: v parse_list_kind (list p.t))
+  (ar: byte_array)
+: STGhost (v (parse_recursive_kind p.parse_header_kind) p.t) opened
+    (aparse p.parse_header al vl `star`
+      aparse (parse_list (parse_recursive p)) ar vr
+    )
+    (fun va -> aparse (parse_recursive p) al va)
+    (AP.adjacent (array_of vl) (array_of vr) /\
+      List.Tot.length vr.contents == p.count vl.contents
+    )
+    (fun va ->
+      AP.merge_into (array_of vl) (array_of vr) (array_of va) /\
+      List.Tot.length vr.contents == p.count vl.contents /\
+      va.contents == p.synth_ (| vl.contents, vr.contents |)
+    )
+= let _ = NL.aparse_list_aparse_nlist (parse_recursive p) (p.count vl.contents) ar in
+  intro_recursive_as_nlist p (p.count vl.contents) al ar
+
+let elim_recursive_as_list_post
+  (p: parse_recursive_param)
+  (va: v (parse_recursive_kind p.parse_header_kind) p.t)
+  (vl: v p.parse_header_kind p.header)
+  (vr: v parse_list_kind (list p.t))
+: GTot prop
+= 
+        AP.merge_into (array_of vl) (array_of vr) (array_of va) /\
+        List.Tot.length vr.contents == p.count vl.contents /\
+        va.contents == p.synth_ (| vl.contents, vr.contents |)
+
+let elim_recursive_as_list
+  (#opened: _)
+  (p: parse_recursive_param)
+  (#va: v (parse_recursive_kind p.parse_header_kind) p.t)
+  (a: byte_array)
+: STGhostT (Ghost.erased byte_array) opened
+    (aparse (parse_recursive p) a va)
+    (fun ar -> exists_ (fun (vl: v p.parse_header_kind p.header) -> exists_ (fun (vr: v parse_list_kind (list p.t)) ->
+      aparse p.parse_header a vl `star`
+      aparse (parse_list (parse_recursive p)) ar vr `star`
+      pure (elim_recursive_as_list_post p va vl vr)
+   )))
+= Classical.forall_intro (parse_recursive_eq p);
+  let _ = rewrite_aparse a (parse_recursive_alt p (parse_recursive p) `parse_synth` p.synth_) in
+  let _ = LPC.elim_synth _ _ a () in
+  let ar = LPC.ghost_split_dtuple2 _ _ a in
+  let _ = gen_elim () in
+  let tag = LPC.ghost_dtuple2_tag _ _ a ar in
+  let _ = gen_elim () in
+  let _ = rewrite_aparse ar (parse_nlist (p.count tag) (parse_recursive p)) in
+  let _ = NL.aparse_nlist_aparse_list (parse_recursive p) (p.count tag) ar in
+  noop ();
+  ar
+
+let elim_recursive_as_nlist_post
+  (p: parse_recursive_param)
+  (va: v (parse_recursive_kind p.parse_header_kind) p.t)
+  (vl: v p.parse_header_kind p.header)
+  (vr: v (parse_nlist_kind (p.count vl.contents) (parse_recursive_kind p.parse_header_kind)) (nlist (p.count vl.contents) p.t))
+: GTot prop
+= 
+        AP.merge_into (array_of vl) (array_of vr) (array_of va) /\
+        va.contents == p.synth_ (| vl.contents, vr.contents |)
+
+#set-options "--ide_id_info_off"
+
+#push-options "--z3rlimit 16"
+
+#restart-solver
+let elim_recursive_as_nlist
+  (#opened: _)
+  (p: parse_recursive_param)
+  (#va: v (parse_recursive_kind p.parse_header_kind) p.t)
+  (a: byte_array)
+: STGhostT (Ghost.erased byte_array) opened
+    (aparse (parse_recursive p) a va)
+    (fun ar -> exists_ (fun vl -> exists_ (fun vr ->
+      aparse p.parse_header a vl `star`
+      aparse (parse_nlist (p.count vl.contents) (parse_recursive p)) ar vr `star`
+      pure (elim_recursive_as_nlist_post p va vl vr)
+    )))
+= let ar = elim_recursive_as_list p a in
+  let _ = gen_elim () in
+  let vl = vpattern_replace (aparse _ a) in
+  let vr = NL.aparse_list_aparse_nlist (parse_recursive p) (p.count vl.contents) ar in
+  intro_pure (elim_recursive_as_nlist_post p va vl vr);
+  noop ();
+  ar
+
+#pop-options
+
+[@@erasable]
+noeq
+type fold_recursive_t
+  (#p: parse_recursive_param)
+  (s: serialize_recursive_param p)
+  (t: Type)
+: Type
+= {
+    step: (t -> p.t -> t);
+    fold: (t -> p.t -> t);
+    prf: (
+      (init: t) ->
+      (x: p.t) ->
+      Lemma
+      (fold init x ==
+        List.Tot.fold_left
+          fold
+          (step init x)
+          (get_children s x) 
+      )
+    );
+  }
+
+let fold_recursive_restore_t
+  (p: parse_recursive_param)
+  (a0: byte_array)
+  (n0: nat)
+  (va0: v (parse_nlist_kind n0 (parse_recursive_kind p.parse_header_kind)) (nlist n0 p.t))
+  (cl: bytes)
+  (n: nat)
+  (ca: nlist n p.t)
+: Tot Type
+= (opened: _) -> 
+  (vl: AP.v byte) ->
+  (va: v (parse_nlist_kind n (parse_recursive_kind p.parse_header_kind)) (nlist n p.t)) ->
+  (a: byte_array) ->
+  STGhost unit opened
+      (AP.arrayptr a0 vl `star` aparse (parse_nlist n (parse_recursive p)) a va)
+      (fun _ -> aparse (parse_nlist n0 (parse_recursive p)) a0 va0)
+      (AP.merge_into (AP.array_of vl) (array_of' va) (array_of' va0) /\
+        AP.contents_of vl == cl /\
+        va.contents == ca)
+      (fun _ -> True)
+
+let intro_exists_fold_recursive_restore
+  (p: parse_recursive_param)
+  (a0: byte_array)
+  (n0: nat)
+  (va0: v (parse_nlist_kind n0 (parse_recursive_kind p.parse_header_kind)) (nlist n0 p.t))
+  (cl: bytes)
+  (n: nat)
+  (ca: nlist n p.t)
+  (phi: fold_recursive_restore_t p a0 n0 va0 cl n ca)
+: Lemma
+  (exists (x: fold_recursive_restore_t p a0 n0 va0 cl n ca) . True)
+= ()
+
+let elim_exists_fold_recursive_restore
+  (#opened: _)
+  (p: parse_recursive_param)
+  (a0: byte_array)
+  (n0: nat)
+  (va0: v (parse_nlist_kind n0 (parse_recursive_kind p.parse_header_kind)) (nlist n0 p.t))
+  (vl: AP.v byte)
+  (n: nat)
+  (va: v (parse_nlist_kind n (parse_recursive_kind p.parse_header_kind)) (nlist n p.t))
+  (a: byte_array)
+: STGhost unit opened
+    (AP.arrayptr a0 vl `star` aparse (parse_nlist n (parse_recursive p)) a va)
+    (fun _ -> aparse (parse_nlist n0 (parse_recursive p)) a0 va0)
+    ((exists (x: fold_recursive_restore_t p a0 n0 va0 (AP.contents_of vl) n va.contents) . True) /\
+      AP.merge_into (AP.array_of vl) (array_of' va) (array_of' va0)
+    )
+    (fun _ -> True)
+= FStar.IndefiniteDescription.indefinite_description_ghost
+    (fold_recursive_restore_t p a0 n0 va0 (AP.contents_of vl) n va.contents)
+    (fun _ -> True)
+    _ _ _
+    a
+
+unfold
+let fold_recursive_invariant_prop0
+  (#p: parse_recursive_param)
+  (s: serialize_recursive_param p)
+  (a0: byte_array)
+  (n0: nat)
+  (va0: v (parse_nlist_kind n0 (parse_recursive_kind p.parse_header_kind)) (nlist n0 p.t))
+  (#t: Type)
+  (fold: fold_recursive_t s t)
+  (init: t)
+  (cont: bool)
+  (vl: _)
+  (n: _)
+  (va: v (parse_nlist_kind (SZ.v n) (parse_recursive_kind p.parse_header_kind)) (nlist (SZ.v n) p.t))
+  (x: _)
+: GTot prop
+=
+      (exists (x: fold_recursive_restore_t p a0 n0 va0 (AP.contents_of vl) (SZ.v n) va.contents) . True) /\
+      List.Tot.fold_left fold.fold init va0.contents == List.Tot.fold_left fold.fold x va.contents /\
+      AP.merge_into (AP.array_of vl) (array_of' va) (array_of' va0) /\
+      cont == (n <> 0sz)
+
+let fold_recursive_invariant_prop
+  (#p: parse_recursive_param)
+  (s: serialize_recursive_param p)
+  (a0: byte_array)
+  (n0: nat)
+  (va0: v (parse_nlist_kind n0 (parse_recursive_kind p.parse_header_kind)) (nlist n0 p.t))
+  (#t: Type)
+  (fold: fold_recursive_t s t)
+  (init: t)
+  (cont: bool)
+  (vl: _)
+  (n: _)
+  (va: v (parse_nlist_kind (SZ.v n) (parse_recursive_kind p.parse_header_kind)) (nlist (SZ.v n) p.t))
+  (x: _)
+: GTot prop
+= fold_recursive_invariant_prop0 s a0 n0 va0 fold init cont vl n va x
+
+[@@__reduce__]
+let fold_recursive_invariant0
+  (#p: parse_recursive_param)
+  (s: serialize_recursive_param p)
+  (a0: byte_array)
+  (n0: nat)
+  (va0: v (parse_nlist_kind n0 (parse_recursive_kind p.parse_header_kind)) (nlist n0 p.t))
+  (pa: R.ref byte_array)
+  (pn: R.ref SZ.t)
+  (#t: Type)
+  (fold: fold_recursive_t s t)
+  (init: t)
+  (q: t -> vprop)
+  (cont: bool)
+: Tot vprop
+= exists_ (fun a -> exists_ (fun vl -> exists_ (fun n -> exists_ (fun va -> exists_ (fun x ->
+    R.pts_to pa full_perm a `star`
+    AP.arrayptr a0 vl `star`
+    R.pts_to pn full_perm n `star`
+    q x `star`
+    aparse (parse_nlist (SZ.v n) (parse_recursive p)) a va `star`
+    pure (fold_recursive_invariant_prop s a0 n0 va0 fold init cont vl n va x)
+  )))))
+
+let fold_recursive_invariant
+  (#p: parse_recursive_param)
+  (s: serialize_recursive_param p)
+  (a0: byte_array)
+  (n0: nat)
+  (va0: v (parse_nlist_kind n0 (parse_recursive_kind p.parse_header_kind)) (nlist n0 p.t))
+  (pa: R.ref byte_array)
+  (pn: R.ref SZ.t)
+  (#t: Type)
+  (fold: fold_recursive_t s t)
+  (init: t)
+  (q: t -> vprop)
+  (cont: bool)
+: Tot vprop
+= fold_recursive_invariant0 s a0 n0 va0 pa pn fold init q cont
+
+let intro_fold_recursive_invariant
+  (#opened: _)
+  (#p: parse_recursive_param)
+  (s: serialize_recursive_param p)
+  (a0: byte_array)
+  (n0: nat)
+  (va0: v (parse_nlist_kind n0 (parse_recursive_kind p.parse_header_kind)) (nlist n0 p.t))
+  (pa: R.ref byte_array)
+  (pn: R.ref SZ.t)
+  (#t: Type)
+  (fold: fold_recursive_t s t)
+  (init: t)
+  (q: t -> vprop)
+  (cont: bool)
+  (a: _)
+  (vl: _)
+  (n: _)
+  (va: _)
+  (x: _)
+: STGhost unit opened
+    (R.pts_to pa full_perm a `star`
+      AP.arrayptr a0 vl `star`
+      R.pts_to pn full_perm n `star`
+      q x `star`
+      aparse (parse_nlist (SZ.v n) (parse_recursive p)) a va
+    )
+    (fun _ -> fold_recursive_invariant s a0 n0 va0 pa pn fold init q cont)
+    (fold_recursive_invariant_prop0 s a0 n0 va0 fold init cont vl n va x)
+    (fun _ -> True)
+= noop ();
+  rewrite
+    (fold_recursive_invariant0 s a0 n0 va0 pa pn fold init q cont)
+    (fold_recursive_invariant s a0 n0 va0 pa pn fold init q cont)
+
+inline_for_extraction
+let size_add_fits
+  (n1 n2: SZ.t)
+  (bound: Ghost.erased SZ.t)
+  (sq: squash (SZ.v n1 + SZ.v n2 <= SZ.v bound))
+: Pure SZ.t
+    (requires True)
+    (ensures (fun y -> SZ.v y == SZ.v n1 + SZ.v n2))
+= n1 `SZ.add` n2
+
+let aparse_nlist_count_le_size
+  (k: parser_kind)
+  (t: Type)
+  (n: nat)
+  (va: v (parse_nlist_kind n k) (nlist n t))
+  (sq: squash (k.parser_kind_low > 0))
+: Tot (squash (n <= AP.length (array_of' va)))
+= ()
+
+let seq_append_injective
+  (#t: Type)
+  (sl1 sl2 sr1 sr2: Seq.seq t)
+: Lemma
+  (requires (
+    (Seq.length sl1 == Seq.length sl2 \/ Seq.length sr1 == Seq.length sr2) /\
+    Seq.append sl1 sr1 == Seq.append sl2 sr2
+  ))
+  (ensures (
+    sl1 `Seq.equal` sl2 /\
+    sr1 `Seq.equal` sr2
+  ))
+= let s = sl1 `Seq.append` sr1 in
+  assert (sl1 `Seq.equal` Seq.slice s 0 (Seq.length sl1));
+  assert (sr1 `Seq.equal` Seq.slice s (Seq.length s - Seq.length sr1) (Seq.length s));
+  Seq.lemma_split s (Seq.length sl1);
+  Seq.lemma_split s (Seq.length s - Seq.length sr1)
+
+let list_fold_left_append
+  (#a #b: Type)
+  (f: a -> b -> Tot a)
+  (l1 l2: list b)
+  (x: a)
+: Tot (squash (List.Tot.fold_left f x (l1 `List.Tot.append` l2) == List.Tot.fold_left f (List.Tot.fold_left f x l1) l2))
+= List.Tot.fold_left_append f l1 l2
+
+let fold_recursive_cons_eq
+  (#p: parse_recursive_param)
+  (s: serialize_recursive_param p)
+  (#t: Type)
+  (fold: fold_recursive_t s t)
+  (init: t)
+  (hd: p.t)
+  (tl: list p.t)
+  (l': list p.t)
+: Lemma
+  (requires (
+    l' == List.Tot.append (get_children s hd) tl
+  ))
+  (ensures (
+    List.Tot.fold_left fold.fold init (hd :: tl) == List.Tot.fold_left fold.fold (fold.step init hd) l'
+  ))
+= fold.prf init hd;
+  list_fold_left_append fold.fold (get_children s hd) tl (fold.step init hd)
+
+let get_children_synth
+  (#p: parse_recursive_param)
+  (s: serialize_recursive_param p)
+  (x: parse_recursive_alt_t p.t p.header p.count)
+: Lemma
+  (get_children s (p.synth_ x) == dsnd x)
+= let y = s.synth_recip (p.synth_ x) in
+  assert (p.synth_ x == p.synth_ y)
+
+#push-options "--z3rlimit 128 --fuel 3 --ifuel 6 --query_stats --split_queries always --z3cliopt smt.arith.nl=false"
+
+#restart-solver
+inline_for_extraction
+let fold_recursive_step
+  (#p: parse_recursive_param u#0 u#0) // gen_elim universe issue
+  (s: serialize_recursive_param p)
+  (w: jumper p.parse_header)
+  (count: jump_recursive_step_count p)
+  (a0: byte_array)
+  (n0: Ghost.erased nat)
+  (va0: v (parse_nlist_kind n0 (parse_recursive_kind p.parse_header_kind)) (nlist n0 p.t))
+  (pa: R.ref byte_array)
+  (pn: R.ref SZ.t)
+  (#t: Type0) // gen_elim universe issue
+  (fold: fold_recursive_t s t)
+  (init: t)
+  (state: t -> vprop)
+  (step: (
+    (x: Ghost.erased t) ->
+    (a: byte_array) ->
+    (va: v (parse_recursive_kind p.parse_header_kind) p.t) ->
+    STT unit
+      (aparse (parse_recursive p) a va `star` state x)
+      (fun _ -> aparse (parse_recursive p) a va `star` state (fold.step x va.contents))
+  ))
+  (_: unit)
+: STT unit
+    (fold_recursive_invariant s a0 n0 va0 pa pn fold init state true)
+    (fun _ -> exists_ (fold_recursive_invariant s a0 n0 va0 pa pn fold init state))
+= rewrite_with_tactic
+    (fold_recursive_invariant s a0 n0 va0 pa pn fold init state true)
+    (fold_recursive_invariant0 s a0 n0 va0 pa pn fold init state true);
+  let _ = gen_elim () in
+  let n = read_replace pn in
+  let n_pred = n `SZ.sub` 1sz in
+  let a = read_replace pa in
+  vpattern_rewrite (fun a -> aparse _ a _) a;
+  let _ = rewrite_aparse a (parse_nlist (SZ.v n) (parse_recursive p)) in
+  let ga3 = NL.elim_nlist_cons (parse_recursive p) (SZ.v n) (SZ.v n_pred) a in
+  let _ = gen_elim () in
+  let x = vpattern_replace_erased state in
+  let va1 = vpattern_replace (aparse (parse_recursive p) a) in
+  let va3 : v _ (nlist (SZ.v n_pred) p.t) = vpattern_replace (aparse (parse_nlist (SZ.v n_pred) (parse_recursive p)) ga3) in
+  step _ a _;
+  let ga2 = elim_recursive_as_nlist p a in
+  let _ = gen_elim () in
+  let va = vpattern_replace (aparse _ a) in
+  let va2 = rewrite_aparse ga2 (parse_nlist (p.count va.contents) (parse_recursive p)) in
+  let _ = aparse_nlist_count_le_size _ _ _ va2 () in
+  noop ();
+  let nl = count a (AP.len (array_of' va2)) in
+  let va2 : v _ (nlist (SZ.v nl) p.t) = rewrite_aparse ga2 (parse_nlist (SZ.v nl) (parse_recursive p)) in
+  let gn' : Ghost.erased nat = Ghost.hide (SZ.v nl + SZ.v n_pred) in
+  noop ();
+  let vr = NL.intro_nlist_sum gn' (parse_recursive p) (SZ.v nl) ga2 (SZ.v n_pred) ga3 in
+  let _ = aparse_nlist_count_le_size _ _ _ vr () in
+  let n' = size_add_fits nl n_pred (AP.len (array_of' vr)) () in
+  noop ();
+  R.write pn n';
+  let vr : v _ (nlist (SZ.v n') p.t) = rewrite_aparse ga2 (parse_nlist (SZ.v n') (parse_recursive p)) in
+  let a2 = hop_aparse_aparse w _ a ga2 in
+  R.write pa a2;
+  let vab = elim_aparse p.parse_header a in
+  let vl = vpattern_replace (AP.arrayptr a0) in
+  let vl' = AP.join a0 a in
+  get_children_synth s (| va.contents, va2.contents |);
+  fold_recursive_cons_eq s fold x va1.contents va3.contents vr.contents;
+  intro_exists_fold_recursive_restore p a0 n0 va0 (AP.contents_of vl') (SZ.v n') vr.contents (fun _ _ _ a2 ->
+    let a = AP.gsplit a0 (AP.len (AP.array_of vl)) in
+    let _ = gen_elim () in
+    let vl_ = vpattern_replace (AP.arrayptr a0) in
+    let vab_ = vpattern_replace (AP.arrayptr a) in
+    seq_append_injective (AP.contents_of vl_) (AP.contents_of vl) (AP.contents_of vab_) (AP.contents_of vab);
+    noop ();
+    let _ = intro_aparse p.parse_header a in
+    let a3 = NL.elim_nlist_sum (SZ.v n') (parse_recursive p) a2 (SZ.v nl) (SZ.v n_pred) in
+    let _ = gen_elim () in
+    let va2_ : v _ (nlist (SZ.v nl) p.t) = vpattern_replace (aparse (parse_nlist (SZ.v nl) (parse_recursive p)) a2) in
+    let va3_ : v _ (nlist (SZ.v n_pred) p.t) = vpattern_replace (aparse (parse_nlist (SZ.v n_pred) (parse_recursive p)) a3) in
+    List.Tot.append_injective va2.contents va2_.contents va3.contents va3_.contents;
+    noop ();
+    let _ = intro_recursive_as_nlist p (SZ.v nl) a a2 in
+    let _ = NL.intro_nlist_cons (SZ.v n) (parse_recursive p) (SZ.v n_pred) a a3 in
+    elim_exists_fold_recursive_restore p a0 n0 va0 _ (SZ.v n) _ a
+  );
+  noop ();
+  intro_fold_recursive_invariant s a0 n0 va0 pa pn fold init state (n' <> 0sz) a2 vl' n' vr _;
+  noop ()
+
+#pop-options
